testcases/printtest/exec_IR.ll
@@ -1,24 +1,21 @@
-; ModuleID = '/home/clexma/Desktop/Disk_D/Tools/SMACK/SmackBasedPrj/build/b-shct3t6y.bc'
+; ModuleID = '/home/clexma/Desktop/Disk_D/Tools/SMACK/SmackBasedPrj/build/b-bnitlbxh.bc'
 source_filename = "llvm-link"
 target datalayout = "e-m:e-p270:32:32-p271:32:32-p272:64:64-i64:64-f80:128-n8:16:32:64-S128"
 target triple = "x86_64-pc-linux-gnu"
 
 ; Function Attrs: noinline nounwind uwtable
-define dso_local i32 @main() #0 !dbg !21 {
-  call void @llvm.dbg.value(metadata i32 11, metadata !24, metadata !DIExpression()), !dbg !25, !verifier.code !26
-  %1 = call noalias i8* @malloc(i64 4) #3, !dbg !27, !verifier.code !26
+define dso_local i32 @main() #0 !dbg !22 {
+  %1 = call noalias i8* @malloc(i64 32) #3, !dbg !25, !verifier.code !26
   %2 = bitcast i8* %1 to i32*, !dbg !27, !verifier.code !26
-  call void @llvm.dbg.value(metadata i32* %2, metadata !28, metadata !DIExpression()), !dbg !25, !verifier.code !26
-  %3 = icmp sgt i32 11, 10, !dbg !29, !verifier.code !26
-  br i1 %3, label %4, label %6, !dbg !31, !verifier.code !26
-
-4:                                                ; preds = %0
-  %5 = bitcast i32* %2 to i8*, !dbg !32, !verifier.code !26
-  call void @free(i8* %5) #3, !dbg !34, !verifier.code !26
-  br label %6, !dbg !35, !verifier.code !26
-
-6:                                                ; preds = %4, %0
-  ret i32 0, !dbg !36, !verifier.code !26
+  call void @llvm.dbg.value(metadata i32* %2, metadata !28, metadata !DIExpression()), !dbg !29, !verifier.code !26
+  %3 = getelementptr inbounds i32, i32* %2, i64 3, !dbg !30, !verifier.code !26
+  store i32 10, i32* %3, align 4, !dbg !31, !verifier.code !26
+  store i32 100, i32* %2, align 4, !dbg !32, !verifier.code !26
+  %4 = getelementptr inbounds i32, i32* %2, i64 3, !dbg !33, !verifier.code !26
+  store i32 11, i32* %4, align 4, !dbg !34, !verifier.code !26
+  %5 = bitcast i32* %2 to i8*, !dbg !35, !verifier.code !26
+  call void @free(i8* %5) #3, !dbg !36, !verifier.code !26
+  ret i32 0, !dbg !37, !verifier.code !26
 }
 
 ; Function Attrs: nounwind readnone speculatable willreturn
@@ -44,43 +41,44 @@ attributes #2 = { nounwind "correctly-rounded-divide-sqrt-fp-math"="false" "disa
 attributes #3 = { nounwind }
 
 !llvm.dbg.cu = !{!0}
-!llvm.ident = !{!17}
-!llvm.module.flags = !{!18, !19, !20}
+!llvm.ident = !{!18}
+!llvm.module.flags = !{!19, !20, !21}
 
-!0 = distinct !DICompileUnit(language: DW_LANG_C99, file: !1, producer: "clang version 10.0.0-4ubuntu1 ", isOptimized: false, runtimeVersion: 0, emissionKind: FullDebug, enums: !2, globals: !3, splitDebugInlining: false, nameTableKind: None)
+!0 = distinct !DICompileUnit(language: DW_LANG_C99, file: !1, producer: "clang version 10.0.0-4ubuntu1 ", isOptimized: false, runtimeVersion: 0, emissionKind: FullDebug, enums: !2, retainedTypes: !3, globals: !6, splitDebugInlining: false, nameTableKind: None)
 !1 = !DIFile(filename: "../testcases/printtest/exec.c", directory: "/home/clexma/Desktop/Disk_D/Tools/SMACK/SmackBasedPrj/build")
 !2 = !{}
-!3 = !{!4, !8, !10, !12}
-!4 = !DIGlobalVariableExpression(var: !5, expr: !DIExpression())
-!5 = distinct !DIGlobalVariable(name: "a", scope: !0, file: !1, line: 14, type: !6, isLocal: false, isDefinition: true)
-!6 = !DIDerivedType(tag: DW_TAG_pointer_type, baseType: !7, size: 64)
-!7 = !DIBasicType(name: "int", size: 32, encoding: DW_ATE_signed)
-!8 = !DIGlobalVariableExpression(var: !9, expr: !DIExpression())
-!9 = distinct !DIGlobalVariable(name: "b", scope: !0, file: !1, line: 14, type: !6, isLocal: false, isDefinition: true)
-!10 = !DIGlobalVariableExpression(var: !11, expr: !DIExpression())
-!11 = distinct !DIGlobalVariable(name: "n", scope: !0, file: !1, line: 15, type: !7, isLocal: false, isDefinition: true)
-!12 = !DIGlobalVariableExpression(var: !13, expr: !DIExpression())
-!13 = distinct !DIGlobalVariable(name: "c", scope: !0, file: !1, line: 17, type: !14, isLocal: false, isDefinition: true)
-!14 = !DICompositeType(tag: DW_TAG_array_type, baseType: !7, size: 320, elements: !15)
-!15 = !{!16}
-!16 = !DISubrange(count: 10)
-!17 = !{!"clang version 10.0.0-4ubuntu1 "}
-!18 = !{i32 7, !"Dwarf Version", i32 4}
-!19 = !{i32 2, !"Debug Info Version", i32 3}
-!20 = !{i32 1, !"wchar_size", i32 4}
-!21 = distinct !DISubprogram(name: "main", scope: !1, file: !1, line: 20, type: !22, scopeLine: 20, spFlags: DISPFlagDefinition, unit: !0, retainedNodes: !2)
-!22 = !DISubroutineType(types: !23)
-!23 = !{!7}
-!24 = !DILocalVariable(name: "a", scope: !21, file: !1, line: 117, type: !7)
-!25 = !DILocation(line: 0, scope: !21)
+!3 = !{!4}
+!4 = !DIDerivedType(tag: DW_TAG_pointer_type, baseType: !5, size: 64)
+!5 = !DIBasicType(name: "int", size: 32, encoding: DW_ATE_signed)
+!6 = !{!7, !9, !11, !13}
+!7 = !DIGlobalVariableExpression(var: !8, expr: !DIExpression())
+!8 = distinct !DIGlobalVariable(name: "a", scope: !0, file: !1, line: 14, type: !4, isLocal: false, isDefinition: true)
+!9 = !DIGlobalVariableExpression(var: !10, expr: !DIExpression())
+!10 = distinct !DIGlobalVariable(name: "b", scope: !0, file: !1, line: 14, type: !4, isLocal: false, isDefinition: true)
+!11 = !DIGlobalVariableExpression(var: !12, expr: !DIExpression())
+!12 = distinct !DIGlobalVariable(name: "n", scope: !0, file: !1, line: 15, type: !5, isLocal: false, isDefinition: true)
+!13 = !DIGlobalVariableExpression(var: !14, expr: !DIExpression())
+!14 = distinct !DIGlobalVariable(name: "c", scope: !0, file: !1, line: 17, type: !15, isLocal: false, isDefinition: true)
+!15 = !DICompositeType(tag: DW_TAG_array_type, baseType: !5, size: 320, elements: !16)
+!16 = !{!17}
+!17 = !DISubrange(count: 10)
+!18 = !{!"clang version 10.0.0-4ubuntu1 "}
+!19 = !{i32 7, !"Dwarf Version", i32 4}
+!20 = !{i32 2, !"Debug Info Version", i32 3}
+!21 = !{i32 1, !"wchar_size", i32 4}
+!22 = distinct !DISubprogram(name: "main", scope: !1, file: !1, line: 20, type: !23, scopeLine: 20, spFlags: DISPFlagDefinition, unit: !0, retainedNodes: !2)
+!23 = !DISubroutineType(types: !24)
+!24 = !{!5}
+!25 = !DILocation(line: 117, column: 20, scope: !22)
 !26 = !{i1 false}
-!27 = !DILocation(line: 118, column: 14, scope: !21)
-!28 = !DILocalVariable(name: "j", scope: !21, file: !1, line: 118, type: !6)
-!29 = !DILocation(line: 119, column: 10, scope: !30)
-!30 = distinct !DILexicalBlock(scope: !21, file: !1, line: 119, column: 8)
-!31 = !DILocation(line: 119, column: 8, scope: !21)
-!32 = !DILocation(line: 120, column: 14, scope: !33)
-!33 = distinct !DILexicalBlock(scope: !30, file: !1, line: 119, column: 15)
-!34 = !DILocation(line: 120, column: 9, scope: !33)
-!35 = !DILocation(line: 121, column: 5, scope: !33)
-!36 = !DILocation(line: 122, column: 1, scope: !21)
+!27 = !DILocation(line: 117, column: 14, scope: !22)
+!28 = !DILocalVariable(name: "j", scope: !22, file: !1, line: 117, type: !4)
+!29 = !DILocation(line: 0, scope: !22)
+!30 = !DILocation(line: 118, column: 8, scope: !22)
+!31 = !DILocation(line: 118, column: 12, scope: !22)
+!32 = !DILocation(line: 119, column: 8, scope: !22)
+!33 = !DILocation(line: 120, column: 8, scope: !22)
+!34 = !DILocation(line: 120, column: 12, scope: !22)
+!35 = !DILocation(line: 121, column: 10, scope: !22)
+!36 = !DILocation(line: 121, column: 5, scope: !22)
+!37 = !DILocation(line: 122, column: 1, scope: !22)
