testcases/printtest/test_with_function_IR.ll
@@ -1,4 +1,4 @@
-; ModuleID = '/home/clexma/Desktop/Disk_D/Tools/SMACK/SmackBasedPrj/build/b-uzteeu2l.bc'
+; ModuleID = '/home/clexma/Desktop/Disk_D/Tools/SMACK/SmackBasedPrj/build/b-csa7rsiw.bc'
 source_filename = "llvm-link"
 target datalayout = "e-m:e-p270:32:32-p271:32:32-p272:64:64-i64:64-f80:128-n8:16:32:64-S128"
 target triple = "x86_64-pc-linux-gnu"
@@ -6,37 +6,85 @@ target triple = "x86_64-pc-linux-gnu"
 ; Function Attrs: nounwind readnone speculatable willreturn
 declare void @llvm.dbg.declare(metadata, metadata, metadata) #0
 
+; Function Attrs: nounwind
+declare dso_local noalias i8* @malloc(i64) #1
+
+; Function Attrs: nounwind
+declare dso_local void @free(i8*) #1
+
 ; Function Attrs: noinline nounwind uwtable
-define internal i32 @recursive(i32 %0) #1 !dbg !11 {
-  call void @llvm.dbg.value(metadata i32 %0, metadata !14, metadata !DIExpression()), !dbg !15, !verifier.code !16
-  %2 = icmp eq i32 %0, 1, !dbg !17, !verifier.code !16
-  br i1 %2, label %3, label %4, !dbg !19, !verifier.code !16
-
-3:                                                ; preds = %1
-  br label %8, !dbg !20, !verifier.code !16
-
-4:                                                ; preds = %1
-  %5 = sub nsw i32 %0, 1, !dbg !21, !verifier.code !16
-  %6 = call i32 @recursive(i32 %5), !dbg !22, !verifier.code !16
-  %7 = add nsw i32 %6, 1, !dbg !23, !verifier.code !16
-  br label %8, !dbg !24, !verifier.code !16
-
-8:                                                ; preds = %4, %3
-  %.0 = phi i32 [ 1, %3 ], [ %7, %4 ], !dbg !25, !verifier.code !16
-  ret i32 %.0, !dbg !26, !verifier.code !16
+define internal void @add_1(i32* %0) #2 !dbg !11 {
+  call void @llvm.dbg.value(metadata i32* %0, metadata !14, metadata !DIExpression()), !dbg !15, !verifier.code !16
+  %2 = load i32, i32* %0, align 4, !dbg !17, !verifier.code !16
+  %3 = add nsw i32 %2, 1, !dbg !17, !verifier.code !16
+  store i32 %3, i32* %0, align 4, !dbg !17, !verifier.code !16
+  ret void, !dbg !18, !verifier.code !16
 }
 
 ; Function Attrs: noinline nounwind uwtable
-define internal void @test_2() #1 !dbg !27 {
-  %1 = call i32 @recursive(i32 2), !dbg !30, !verifier.code !16
-  call void @llvm.dbg.value(metadata i32 %1, metadata !31, metadata !DIExpression()), !dbg !32, !verifier.code !16
-  ret void, !dbg !33, !verifier.code !16
+define internal void @add_2(i32* %0) #2 !dbg !19 {
+  call void @llvm.dbg.value(metadata i32* %0, metadata !20, metadata !DIExpression()), !dbg !21, !verifier.code !16
+  %2 = load i32, i32* %0, align 4, !dbg !22, !verifier.code !16
+  %3 = add nsw i32 %2, 2, !dbg !22, !verifier.code !16
+  store i32 %3, i32* %0, align 4, !dbg !22, !verifier.code !16
+  ret void, !dbg !23, !verifier.code !16
 }
 
 ; Function Attrs: noinline nounwind uwtable
-define dso_local i32 @main() #1 !dbg !34 {
-  call void @test_2(), !dbg !37, !verifier.code !16
-  ret i32 0, !dbg !38, !verifier.code !16
+define internal void @test_3() #2 !dbg !24 {
+  %1 = call noalias i8* @malloc(i64 8) #3, !dbg !27, !verifier.code !16
+  %2 = bitcast i8* %1 to i32*, !dbg !28, !verifier.code !16
+  call void @llvm.dbg.value(metadata i32* %2, metadata !29, metadata !DIExpression()), !dbg !30, !verifier.code !16
+  %3 = getelementptr inbounds i32, i32* %2, i64 1, !dbg !31, !verifier.code !16
+  store i32 0, i32* %3, align 4, !dbg !32, !verifier.code !16
+  %4 = getelementptr inbounds i32, i32* %2, i64 0, !dbg !33, !verifier.code !16
+  store i32 0, i32* %4, align 4, !dbg !34, !verifier.code !16
+  call void @add_1(i32* %2), !dbg !35, !verifier.code !16
+  %5 = getelementptr inbounds i32, i32* %2, i64 1, !dbg !36, !verifier.code !16
+  call void @add_2(i32* %5), !dbg !37, !verifier.code !16
+  call void @llvm.dbg.value(metadata i32 0, metadata !38, metadata !DIExpression()), !dbg !30, !verifier.code !16
+  %6 = call noalias i8* @malloc(i64 12) #3, !dbg !39, !verifier.code !16
+  %7 = bitcast i8* %6 to i32*, !dbg !40, !verifier.code !16
+  call void @llvm.dbg.value(metadata i32* %7, metadata !41, metadata !DIExpression()), !dbg !30, !verifier.code !16
+  call void @llvm.dbg.value(metadata i32 0, metadata !42, metadata !DIExpression()), !dbg !44, !verifier.code !16
+  call void @llvm.dbg.value(metadata i32 0, metadata !38, metadata !DIExpression()), !dbg !30, !verifier.code !16
+  br label %8, !dbg !45, !verifier.code !16
+
+8:                                                ; preds = %0
+  call void @llvm.dbg.value(metadata i32 0, metadata !42, metadata !DIExpression()), !dbg !44, !verifier.code !16
+  call void @llvm.dbg.value(metadata i32 0, metadata !38, metadata !DIExpression()), !dbg !30, !verifier.code !16
+  %9 = load i32, i32* %2, align 4, !dbg !46, !verifier.code !16
+  call void @llvm.dbg.value(metadata i32 %9, metadata !38, metadata !DIExpression()), !dbg !30, !verifier.code !16
+  br label %10, !dbg !49, !verifier.code !16
+
+10:                                               ; preds = %8
+  call void @llvm.dbg.value(metadata i32 1, metadata !42, metadata !DIExpression()), !dbg !44, !verifier.code !16
+  call void @llvm.dbg.value(metadata i32 %9, metadata !38, metadata !DIExpression()), !dbg !30, !verifier.code !16
+  %11 = getelementptr inbounds i32, i32* %2, i64 1, !dbg !46, !verifier.code !16
+  %12 = load i32, i32* %11, align 4, !dbg !46, !verifier.code !16
+  %13 = add nsw i32 %9, %12, !dbg !50, !verifier.code !16
+  call void @llvm.dbg.value(metadata i32 %13, metadata !38, metadata !DIExpression()), !dbg !30, !verifier.code !16
+  br label %17, !dbg !49, !verifier.code !16
+
+14:                                               ; preds = %17
+  %15 = bitcast i32* %7 to i8*, !dbg !51, !verifier.code !16
+  call void @free(i8* %15) #3, !dbg !54, !verifier.code !16
+  br label %16, !dbg !55, !verifier.code !16
+
+16:                                               ; preds = %14, %17
+  ret void, !dbg !56, !verifier.code !16
+
+17:                                               ; preds = %10
+  call void @llvm.dbg.value(metadata i32 2, metadata !42, metadata !DIExpression()), !dbg !44, !verifier.code !16
+  call void @llvm.dbg.value(metadata i32 %13, metadata !38, metadata !DIExpression()), !dbg !30, !verifier.code !16
+  %18 = icmp eq i32 %13, 3, !dbg !57, !verifier.code !16
+  br i1 %18, label %14, label %16, !dbg !58, !verifier.code !16
+}
+
+; Function Attrs: noinline nounwind uwtable
+define dso_local i32 @main() #2 !dbg !59 {
+  call void @test_3(), !dbg !62, !verifier.code !16
+  ret i32 0, !dbg !63, !verifier.code !16
 }
 
 ; Function Attrs: nounwind readnone speculatable willreturn
@@ -48,7 +96,9 @@ entry:
 }
 
 attributes #0 = { nounwind readnone speculatable willreturn }
-attributes #1 = { noinline nounwind uwtable "correctly-rounded-divide-sqrt-fp-math"="false" "disable-tail-calls"="false" "frame-pointer"="all" "less-precise-fpmad"="false" "min-legal-vector-width"="0" "no-infs-fp-math"="false" "no-jump-tables"="false" "no-nans-fp-math"="false" "no-signed-zeros-fp-math"="false" "no-trapping-math"="false" "stack-protector-buffer-size"="8" "target-cpu"="x86-64" "target-features"="+cx8,+fxsr,+mmx,+sse,+sse2,+x87" "unsafe-fp-math"="false" "use-soft-float"="false" }
+attributes #1 = { nounwind "correctly-rounded-divide-sqrt-fp-math"="false" "disable-tail-calls"="false" "frame-pointer"="all" "less-precise-fpmad"="false" "no-infs-fp-math"="false" "no-nans-fp-math"="false" "no-signed-zeros-fp-math"="false" "no-trapping-math"="false" "stack-protector-buffer-size"="8" "target-cpu"="x86-64" "target-features"="+cx8,+fxsr,+mmx,+sse,+sse2,+x87" "unsafe-fp-math"="false" "use-soft-float"="false" }
+attributes #2 = { noinline nounwind uwtable "correctly-rounded-divide-sqrt-fp-math"="false" "disable-tail-calls"="false" "frame-pointer"="all" "less-precise-fpmad"="false" "min-legal-vector-width"="0" "no-infs-fp-math"="false" "no-jump-tables"="false" "no-nans-fp-math"="false" "no-signed-zeros-fp-math"="false" "no-trapping-math"="false" "stack-protector-buffer-size"="8" "target-cpu"="x86-64" "target-features"="+cx8,+fxsr,+mmx,+sse,+sse2,+x87" "unsafe-fp-math"="false" "use-soft-float"="false" }
+attributes #3 = { nounwind }
 
 !llvm.dbg.cu = !{!0}
 !llvm.ident = !{!7}
@@ -65,31 +115,56 @@ attributes #1 = { noinline nounwind uwtable "correctly-rounded-divide-sqrt-fp-ma
 !8 = !{i32 7, !"Dwarf Version", i32 4}
 !9 = !{i32 2, !"Debug Info Version", i32 3}
 !10 = !{i32 1, !"wchar_size", i32 4}
-!11 = distinct !DISubprogram(name: "recursive", scope: !1, file: !1, line: 37, type: !12, scopeLine: 37, flags: DIFlagPrototyped, spFlags: DISPFlagDefinition, unit: !0, retainedNodes: !2)
+!11 = distinct !DISubprogram(name: "add_1", scope: !1, file: !1, line: 50, type: !12, scopeLine: 50, flags: DIFlagPrototyped, spFlags: DISPFlagDefinition, unit: !0, retainedNodes: !2)
 !12 = !DISubroutineType(types: !13)
-!13 = !{!5, !5}
-!14 = !DILocalVariable(name: "n", arg: 1, scope: !11, file: !1, line: 37, type: !5)
+!13 = !{null, !4}
+!14 = !DILocalVariable(name: "p", arg: 1, scope: !11, file: !1, line: 50, type: !4)
 !15 = !DILocation(line: 0, scope: !11)
 !16 = !{i1 false}
-!17 = !DILocation(line: 38, column: 11, scope: !18)
-!18 = distinct !DILexicalBlock(scope: !11, file: !1, line: 38, column: 9)
-!19 = !DILocation(line: 38, column: 9, scope: !11)
-!20 = !DILocation(line: 38, column: 17, scope: !18)
-!21 = !DILocation(line: 39, column: 29, scope: !18)
-!22 = !DILocation(line: 39, column: 17, scope: !18)
-!23 = !DILocation(line: 39, column: 34, scope: !18)
-!24 = !DILocation(line: 39, column: 10, scope: !18)
-!25 = !DILocation(line: 0, scope: !18)
-!26 = !DILocation(line: 40, column: 1, scope: !11)
-!27 = distinct !DISubprogram(name: "test_2", scope: !1, file: !1, line: 42, type: !28, scopeLine: 42, spFlags: DISPFlagDefinition, unit: !0, retainedNodes: !2)
-!28 = !DISubroutineType(types: !29)
-!29 = !{null}
-!30 = !DILocation(line: 43, column: 13, scope: !27)
-!31 = !DILocalVariable(name: "t", scope: !27, file: !1, line: 43, type: !5)
-!32 = !DILocation(line: 0, scope: !27)
-!33 = !DILocation(line: 48, column: 1, scope: !27)
-!34 = distinct !DISubprogram(name: "main", scope: !1, file: !1, line: 131, type: !35, scopeLine: 131, spFlags: DISPFlagDefinition, unit: !0, retainedNodes: !2)
-!35 = !DISubroutineType(types: !36)
-!36 = !{!5}
-!37 = !DILocation(line: 134, column: 5, scope: !34)
-!38 = !DILocation(line: 139, column: 5, scope: !34)
+!17 = !DILocation(line: 51, column: 10, scope: !11)
+!18 = !DILocation(line: 52, column: 1, scope: !11)
+!19 = distinct !DISubprogram(name: "add_2", scope: !1, file: !1, line: 54, type: !12, scopeLine: 54, flags: DIFlagPrototyped, spFlags: DISPFlagDefinition, unit: !0, retainedNodes: !2)
+!20 = !DILocalVariable(name: "p", arg: 1, scope: !19, file: !1, line: 54, type: !4)
+!21 = !DILocation(line: 0, scope: !19)
+!22 = !DILocation(line: 55, column: 8, scope: !19)
+!23 = !DILocation(line: 56, column: 1, scope: !19)
+!24 = distinct !DISubprogram(name: "test_3", scope: !1, file: !1, line: 58, type: !25, scopeLine: 58, spFlags: DISPFlagDefinition, unit: !0, retainedNodes: !2)
+!25 = !DISubroutineType(types: !26)
+!26 = !{null}
+!27 = !DILocation(line: 59, column: 20, scope: !24)
+!28 = !DILocation(line: 59, column: 14, scope: !24)
+!29 = !DILocalVariable(name: "a", scope: !24, file: !1, line: 59, type: !4)
+!30 = !DILocation(line: 0, scope: !24)
+!31 = !DILocation(line: 60, column: 12, scope: !24)
+!32 = !DILocation(line: 60, column: 17, scope: !24)
+!33 = !DILocation(line: 60, column: 5, scope: !24)
+!34 = !DILocation(line: 60, column: 10, scope: !24)
+!35 = !DILocation(line: 61, column: 5, scope: !24)
+!36 = !DILocation(line: 62, column: 13, scope: !24)
+!37 = !DILocation(line: 62, column: 5, scope: !24)
+!38 = !DILocalVariable(name: "sum", scope: !24, file: !1, line: 63, type: !5)
+!39 = !DILocation(line: 64, column: 21, scope: !24)
+!40 = !DILocation(line: 64, column: 14, scope: !24)
+!41 = !DILocalVariable(name: "p", scope: !24, file: !1, line: 64, type: !4)
+!42 = !DILocalVariable(name: "i", scope: !43, file: !1, line: 65, type: !5)
+!43 = distinct !DILexicalBlock(scope: !24, file: !1, line: 65, column: 5)
+!44 = !DILocation(line: 0, scope: !43)
+!45 = !DILocation(line: 65, column: 5, scope: !43)
+!46 = !DILocation(line: 66, column: 16, scope: !47)
+!47 = distinct !DILexicalBlock(scope: !48, file: !1, line: 65, column: 34)
+!48 = distinct !DILexicalBlock(scope: !43, file: !1, line: 65, column: 5)
+!49 = !DILocation(line: 67, column: 5, scope: !47)
+!50 = !DILocation(line: 66, column: 13, scope: !47)
+!51 = !DILocation(line: 69, column: 14, scope: !52)
+!52 = distinct !DILexicalBlock(scope: !53, file: !1, line: 68, column: 19)
+!53 = distinct !DILexicalBlock(scope: !24, file: !1, line: 68, column: 9)
+!54 = !DILocation(line: 69, column: 9, scope: !52)
+!55 = !DILocation(line: 70, column: 5, scope: !52)
+!56 = !DILocation(line: 71, column: 1, scope: !24)
+!57 = !DILocation(line: 68, column: 13, scope: !53)
+!58 = !DILocation(line: 68, column: 9, scope: !24)
+!59 = distinct !DISubprogram(name: "main", scope: !1, file: !1, line: 131, type: !60, scopeLine: 131, spFlags: DISPFlagDefinition, unit: !0, retainedNodes: !2)
+!60 = !DISubroutineType(types: !61)
+!61 = !{!5}
+!62 = !DILocation(line: 136, column: 5, scope: !59)
+!63 = !DILocation(line: 140, column: 5, scope: !59)
